Post conditions and MAYCHANGE for an AES block encryption proof.

arm/proofs/aes_encrypt.ml
@@ -20,7 +20,7 @@ let aes256_encrypt_mc = define_assert_from_elf "aes256_encrypt_mc" "arm/aes-xts/
   0x54ffff2c;       (* arm_BGT (word 2097124) *)
   0x4e284806;       (* arm_AESE Q6 Q0 *)
   0x4e2868c6;       (* arm_AESMC Q6 Q6 *)
-  0x4c407880;       (* arm_LDR Q0 X4 No_Offset *)
+  0x4c407840;       (* arm_LDR Q0 X2 No_Offset *)
   0x4e284826;       (* arm_AESE Q6 Q1 *)
   0x6e201cc6;       (* arm_EOR_VEC Q6 Q6 Q0 128 *)
   0x4c007806        (* arm_STR Q6 X0 No_Offset *)
@@ -29,37 +29,41 @@ let aes256_encrypt_mc = define_assert_from_elf "aes256_encrypt_mc" "arm/aes-xts/
 let AES256_ENCRYPT_EXEC = ARM_MK_EXEC_RULE aes256_encrypt_mc;;
 
 (* TODO: Could this be better? read(memory :> bytes(key, 240) = all_k) *)
+
 let AES256_ENCRYPT_CORRECT = prove(
-  `!out in key ib k0 k1 k2 k3 k4 k5 k6 k7 k8 k9 k10 k11 k12 k13 k14 pc.
-    nonoverlapping (word pc,LENGTH aes256_encrypt_mc) (out,16)
+  `!ciphertext plaintext key ib k0 k1 k2 k3 k4 k5 k6 k7 k8 k9 k10 k11 k12 k13 k14 pc.
+    nonoverlapping (word pc,LENGTH aes256_encrypt_mc) (ciphertext,16)
     ==> ensures arm
       // precondition
       (\s. aligned_bytes_loaded s (word pc) aes256_encrypt_mc /\
            read PC s = word pc /\
-           C_ARGUMENTS [out; in; key] s /\
-           read(memory :> bytes(in, 16)) s = ib /\
-           read(memory :> bytes(word_add key (word 240), 4)) = word 13 /\
-           read(memory :> bytes(key, 16)) = k0 /\
-           read(memory :> bytes((word_add key (word 16)), 16)) = k1 /\
-           read(memory :> bytes((word_add key (word 32)), 16)) = k2 /\
-           read(memory :> bytes((word_add key (word 48)), 16)) = k3 /\
-           read(memory :> bytes((word_add key (word 64)), 16)) = k4 /\
-           read(memory :> bytes((word_add key (word 80)), 16)) = k5 /\
-           read(memory :> bytes((word_add key (word 96)), 16)) = k6 /\
-           read(memory :> bytes((word_add key (word 112)), 16)) = k7 /\
-           read(memory :> bytes((word_add key (word 128)), 16)) = k8 /\
-           read(memory :> bytes((word_add key (word 144)), 16)) = k9 /\
-           read(memory :> bytes((word_add key (word 160)), 16)) = k10 /\
-           read(memory :> bytes((word_add key (word 176)), 16)) = k11 /\
-           read(memory :> bytes((word_add key (word 192)), 16)) = k12 /\
-           read(memory :> bytes((word_add key (word 208)), 16)) = k13 /\
-           read(memory :> bytes((word_add key (word 224)), 16)) = k14)
+           C_ARGUMENTS [ciphertext; plaintext; key] s /\
+           read(memory :> bytes(plaintext, 16)) s = ib /\
+           read(memory :> bytes(word_add key (word 240), 4)) s = 14 /\
+           read(memory :> bytes128 key) s = k0 /\
+           read(memory :> bytes128 (word_add key (word 16))) s = k1 /\
+           read(memory :> bytes128 (word_add key (word 32))) s = k2 /\
+           read(memory :> bytes128 (word_add key (word 48))) s = k3 /\
+           read(memory :> bytes128 (word_add key (word 64))) s = k4 /\
+           read(memory :> bytes128 (word_add key (word 80))) s = k5 /\
+           read(memory :> bytes128 (word_add key (word 96))) s = k6 /\
+           read(memory :> bytes128 (word_add key (word 112))) s = k7 /\
+           read(memory :> bytes128 (word_add key (word 128))) s = k8 /\
+           read(memory :> bytes128 (word_add key (word 144))) s = k9 /\
+           read(memory :> bytes128 (word_add key (word 160))) s = k10 /\
+           read(memory :> bytes128 (word_add key (word 176))) s = k11 /\
+           read(memory :> bytes128 (word_add key (word 192))) s = k12 /\
+           read(memory :> bytes128 (word_add key (word 208))) s = k13 /\
+           read(memory :> bytes128 (word_add key (word 224))) s = k14
+      )
       // postcondition
       // TODO: Nevine will figure out the post condition for output
       // hint: use the aes256_encrypt from aes_encrypt_spec
       (\s. read PC s = word (pc + LENGTH aes256_encrypt_mc) /\
-           )
-      // MAYCHANGE
-      ()`,
+           read(memory :> bytes128 ciphertext) s =
+              aes256_encrypt (word ib)
+                [k0; k1; k2; k3; k4; k5; k6; k7; k8; k9; k10; k11; k12; k13; k14]
+      )
+      (MAYCHANGE [PC;X2],, MAYCHANGE [Q0;Q1;Q6],, MAYCHANGE [W6])`,
   CHEAT_TAC
-)
+);;
